Sketches of a proof

compiler/scheme/proofs/scheme_compileCorrectScript.sml
@@ -100,20 +100,32 @@ Proof
   >> simp[letinit_ml_def, do_con_check_def, nsLookup_def]
 QED
 
+Definition scheme_out_oracle_def:
+  scheme_out_oracle =
+    <| oracle      := (λffi_name _ _ _.
+                         (* accepts calls to scheme_out *)
+                         if ffi_name = ExtCall "scheme_out"
+                         then Oracle_return () [] (* returns empty *)
+                         else Oracle_final FFI_failed)
+     ; ffi_state   := ()
+     ; io_events   := []  |>  :unit ffi_state
+End
+
 Theorem scheme_semantics_preservation_terminates:
-  ! prog cml_prog v st env (ffi :'ffi ffi_state) .
+  ∀ prog cml_prog v st env .
     scheme_semantics_prog prog (STerminate v) /\
     static_scope_check prog = INR prog /\
     codegen prog = INR cml_prog
     ==>
-    semantics_prog (init_state ffi) init_env cml_prog (Terminate Success [v_to_string v])
+    semantics_prog (init_state scheme_out_oracle) init_env cml_prog
+                   (Terminate Success [v_to_string v])
 Proof
   simp[semantics_prog_def, scheme_semantics_prog_def]
   >> simp[static_scope_check_def]
   >> simp_tac std_ss [codegen_def]
   >> simp[evaluate_prog_with_clock_def]
   >> rpt strip_tac
-  >> qspec_then `ffi` assume_tac scheme_init_evaluate_dec
+  >> qspec_then `scheme_out_oracle` assume_tac scheme_init_evaluate_dec
   >> gvs[]
   >> qrefine `ck1 + k`
   >> gvs[scheme_init_def]
@@ -146,12 +158,14 @@ Proof
   >> simp[Ntimes evaluate_def 2, nsOptBind_def]
 
   >> gvs[scheme_semanticsTheory.steps_def]
-  >> drule_then assume_tac value_terminating
+  >> drule_then assume_tac (value_terminating |> INST_TYPE [“:'ffi”|->“:unit”])
+
   >> gvs[Once cont_rel_cases, Once valid_state_cases]
   >> gvs[Once valid_cont_cases, can_lookup_cases, FEVERY_FEMPTY]
   >> gvs[Once cps_rel_cases]
   >> qmatch_goalsub_abbrev_tac `evaluate _ newenv [_]`
-  >> first_x_assum $ qspecl_then [`scheme_to_cake_env_st_1 ffi`, `newenv`] assume_tac
+  >> first_x_assum $ qspecl_then
+       [`scheme_to_cake_env_st_1 scheme_out_oracle`, `newenv`] assume_tac
   >> unabbrev_all_tac
   >> gvs[scheme_init_st_defs]
   >> gvs[scheme_env_sub, scheme_runtime_funs_def, basis_scheme_env]
@@ -192,8 +206,13 @@ Proof
   >> simp[evaluate_match_def, can_pmatch_all_def, pmatch_def,
     nsLookup_def, same_type_def, same_ctor_def, pat_bindings_def]
   >> simp[Ntimes evaluate_def 4, do_app_def, store_alloc_def, store_lookup_def,
-    EL_APPEND_EQN, call_FFI_def, store_assign_def, store_v_same_type_def]
-  >> cheat (*seems to depend on the ffi oracle here*)
+    EL_APPEND_EQN, call_FFI_def, store_assign_def, store_v_same_type_def,
+    scheme_out_oracle_def]
+  >> fs [combine_dec_result_def,v_to_string_def]
+  >> gvs [bool_val_rel_cases,pmatch_def,nsLookup_def,same_type_def,same_ctor_def]
+  >> simp[Ntimes evaluate_def 4, do_app_def, store_alloc_def, store_lookup_def,
+    EL_APPEND_EQN, call_FFI_def, store_assign_def, store_v_same_type_def,
+    scheme_out_oracle_def,v_to_string_def]
 QED
 
 Theorem imp_semantics_prog:
